Progress on the tutorial.

tutorial/tutorial.v
@@ -1,10 +1,16 @@
+Set Warnings "-require-in-section". (* .none *)
+
 (*|
 =====================
 Hoare Logic for OCaml
 =====================
 |*)
 
-Require Import base lang free eval step safe wp wp_tactics encode. (* .none *)
+Section Eval. (* .none *)
+Require Import base lang free eval. (* .none *)
+
+Notation ε := EnvNil. (* .none *)
+Notation int := int.int. (* .none *)
 
 (*|
 -----------
@@ -18,7 +24,7 @@ of type `expr`. For instance, the following expression represents the
 OCaml expression :code:`24 + 18`:
 |*)
 
-Definition example : expr :=
+Definition add_24_plus_18 : expr :=
   EIntAdd (EInt 24) (EInt 18).
 
 (*|
@@ -64,16 +70,245 @@ We define the semantics of OCaml by implementing an *interpreter* of
 OCaml programs inside Coq. We want this interpreter to be a classic
 environment-based interpreter: when given an environment `η` and an
 expression `e`, it should compute a value `v`.
+|*)
 
+(*|
 *Values* have their own syntactic category: they are not a subset of
 expressions. For instance, a closure is a value, not an expression.
+|*)
 
+Print val.
+
+(*|
 An *environment* is a mapping of variables to values. It is represented
 in Coq as an association list. Because a closure captures an environment,
 the syntactic categories of values and environments are mutually recursive.
 |*)
 
-Print val.
+Print env.
+
+(*|
+---------------------
+A Monadic Interpreter
+---------------------
+|*)
+
+(*|
+OCaml is an effectful programming language: an OCaml program can
+exhibit a variety a side effects. For instance, a program can diverge,
+that is, run forever. A program can have observable side effects, such
+as mutating heap-allocated objects or performing input/output actions.
+A program can behave in a non-deterministic manner, either because of
+its interaction with the operating system, or due to intrinsic
+non-determinism (some OCaml constructs have unspecified evaluation
+order).
+|*)
+
+(*|
+For these reasons, the interpreter cannot be expected to be a
+function of type `env → expr → val`. That would imply that
+interpretation is deterministic and always terminates.
+Instead, the interpreter must be a *monadic* interpreter:
+|*)
+
+Check eval. (* .unfold *)
+
+(*|
+The term `eval η e` has type `free val`,
+where `free` is a *monad*.
+This means that `eval η e` is
+an effectful *computation* which may diverge,
+may behave in a non-deterministic manner, and
+may eventually produce a value.
+
+For instance, evaluating the OCaml expression :code:`42`
+in the empty environment `ε`
+yields the OCaml value :code:`42`:
+|*)
+
+Eval cbn in (eval ε (EInt 42)). (* .unfold *)
+
+(*|
+Coq finds that this computation is equal to
+`ret (VInt (int.repr 42))`.
+
+The data constructor `ret` is the `return` combinator
+of the monad. Its presence means that Coq has been able
+to fully evaluate this computation, whose final result
+is the value `VInt (int.repr 42)`.
+|*)
+
+Check @ret. (* .unfold *)
+
+(*|
+The tag `VInt` identifies an integer value. Its payload,
+`int.repr 42`, is a machine integer.
+OCaml has integers of a limited bit width.
+The projection `int.repr` maps the type `Z` of ideal integers
+into the finite type `int` of the signed machine integers.
+
+|*)
+
+Check int.repr. (* .unfold *)
+
+(*|
+The interpreter is defined in a straightforward way.
+It could be taught in an introductory course on
+programming language implementation.
+Yet, this interpreter plays an important role for us:
+it serves as our definition of the semantics of OCaml
+and as a basis for the program verification system
+that we wish to set up.
+|*)
+
+(*|
+The following equation highlights one case in the definition of `eval`,
+namely the case of the `if/then/else` construct. To evaluate the OCaml
+expression :code:`if e then e1 else e2`, the interpreter first
+evaluates `e` and checks that its result is a Boolean value `VBool b`.
+Then, depending on `b`, it evaluates either `e1` or `e2`.
+Because `e`, `e1`, and `e2` are subexpressions of the expression
+:code:`if e then e1 else e2`, Coq recognizes that
+it is permitted for `eval` to recursively invoke itself.
+|*)
+
+Goal ∀ η e e1 e2,
+  eval η (EIfThenElse e e1 e2) =
+    b ← as_bool (eval η e) ;
+    if (b : bool) then eval η e1 else eval η e2. (* .no-goals *)
+Proof. (* .none *)
+  reflexivity. (* .none *)
+Qed. (* .none *)
+
+(*|
+That said, there are places in the definition of `eval`
+where we would like to recursively invoke `eval`
+but that is not permitted by Coq.
+An example appears in the case of `while` loops:
+|*)
+
+Goal ∀ η e body,
+  eval η (EWhile e body) =
+    b ← as_bool (eval η e) ;
+    if (b : bool) then
+      _ ← eval η body ;
+      stop Eval (η, EWhile e body)
+    else
+      ok. (* .no-goals *)
+Proof. (* .none *)
+  reflexivity. (* .none *)
+Qed. (* .none *)
+
+(*|
+After executing the loop body by calling `eval η body`,
+we would like to execute the loop again.
+This could be done by invoking `eval η (EWhile e body)`,
+but such a recursive call is not permitted.
+Instead, the interpreter *stops*
+with a request for a recursive invocation of `eval`.
+The monadic combinator `stop` expresses such a request.
+
+This request is intended to be serviced by a scheduler
+which supervises the execution of the interpreter.
+It is up to the scheduler to step into the recursive call
+and resume the execution of the interpreter.
+
+Another interesting monadic combinator is `par`,
+a binary combinator that allows two computations
+to be executed in parallel.
+This combinator is typically used in places where
+OCaml has unspecified evaluation order.
+For instance, here is how an OCaml function application :code:`e1 e2`
+is evaluated:
+|*)
+
+Goal ∀ η e1 e2,
+  eval η (EApp e1 e2) =
+    '(v1, v2) ← par (eval η e1) (eval η e2) ;
+    call v1 v2. (* .no-goals *)
+Proof. (* .none *)
+  reflexivity. (* .none *)
+Qed. (* .none *)
+
+(*|
+The recursive calls `eval η e1` and `eval η e2` are executed in parallel.
+If and once these calls yield two values `v1` and `v2`,
+then the auxiliary function `call` (not shown)
+is used to interpret the application of the function `v1`
+to the argument `v2`.
+The use of `par` reflects the fact that the definition of OCaml
+does not specify whether `e1` is evaluated before `e2` is evaluated,
+or `e2` is evaluated before `e1` is evaluated, or the two evaluations
+may be interleaved.
+
+Because we choose a pessimistic semantics
+(that is, a non-deterministic semantics),
+a programmer who reasons about a function application :code:`e1 e2`
+must prove that there is no interference
+between `e1` and `e2`. This is done by applying
+the parallel composition rule
+of concurrent separation logic.
+
+Interpreting an addition expression :code:`e1 + e2`
+also involves a parallel composition:
+|*)
+
+Goal ∀ η e1 e2,
+  eval η (EIntAdd e1 e2) =
+    '(i1, i2) ← par (as_int (eval η e1)) (as_int (eval η e2)) ;
+    ret (VInt (int.add i1 i2)). (* .no-goals *)
+Proof. (* .none *)
+  reflexivity. (* .none *)
+Qed. (* .none *)
+
+(*|
+The reader may wonder how Coq can execute a parallel composition.
+The answer is, it cannot: when the interpreter encounters a `par` combinator,
+it stops. It is then up to the scheduler to take control,
+to decide what step to take next,
+and to resume the interpreter.
+
+This can be observed by asking Coq to evaluate the OCaml expression
+`24 + 18`:
+|*)
+
+Eval cbn in (eval ε add_24_plus_18). (* .unfold *)
+
+(*|
+The interpreter hits a `Par` combinator whose branches are
+`ret (int.repr 24)` and `ret (int.repr 18)`
+and whose continuation is
+`(λ '(i1, i2), ret (VInt (int.add i1 i2)))`.
+|*)
+
+(*|
+To understand how the `stop` and `par` combinators work,
+one must examine how computations are represented
+and how the scheduler is implemented.
+We do so in the next two sections.
+|*)
+
+End Eval. (* .none *)
+
+(*|
+---------
+The Monad
+---------
+|*)
+
+Section Free. (* .none *)
+Require Import base lang free. (* .none *)
+
+Print free. (* .unfold *)
+
+End Free. (* .none *)
+
+(*|
+-------------
+The Scheduler
+-------------
+|*)
+
 
 (*|
 |*)
